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1 Experimental Setup

Imagine you want to measure the flow rate of water out of
a faucet, but your flowmeter is broken. Quick on your feet,
you devise a simple experiment using a graduate cylinder and
wrist watch. The average flow rate is:

F =
Vf − V0

tf − t0
(1)

where V0 is the volume in the cylinder at time t0. You measure
Vf and tf after some time has elapsed.

2 Error Propagation

Your graduated cylinder only measures to the nearest 0.1 mL
and holds a maximum of 50 mL. Your analog wristwatch has
a seconds hand. Based on this, you reason that σV = 0.1 mL
(same for both volume measurements), σt = 1 s (same for both time measurements), and
σV,t = 0 (i.e., the measurement errors are NOT correlated). Although you could conduct
many experiments to estimate σV , σt, and σV,t, you think it is wise to approximate the error
level in F after taking only a few measurements. Here are the data for your first trial:

V0 t0 Vf tf

5.3 mL 1:01:04 49.2 mL 1:01:56
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2.a Approach 1

Which error propagation formula to use? You decide to decompose (1) into two subtraction
steps and one division step:

∆t := tf − t0, ∆V := Vf − V0, F =
∆V

∆t
(2)

where ∆V and ∆t are intermediate variables. You then apply the subtraction error propaga-
tion formula to calculate σ∆V and σ∆t.

σ∆V =
√
σ2
V + σ2

V =
√

2 σV

σ∆t =
√
σ2
t + σ2

t =
√

2 σt

Next, apply the division error propagation formula to estimate σF :

σ2
F ≈ F 2

[(σ∆V

∆V

)2

+
(σ∆t

∆t

)2
]

≈ F 2

[
2
( σV

∆V

)2

+ 2
( σt

∆t

)2
]
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2.b Approach 2

What about the general error propagation formula,

σ2
Z ≈

∣∣∣∣ ∂g∂X
∣∣∣∣2 · σ2

X +

∣∣∣∣ ∂g∂Y
∣∣∣∣2 · σ2

Y + 2 · ∂g
∂X
· ∂g
∂Y
· σX,Y (3)

where Z = g(X, Y ) and g(·) is a differentiable function? You apply this formula to (1). Start
by calculating the partial derivatives ∂F

∂Vf
, ∂F
∂V0

, ∂F
∂tf

, ∂F
∂t0

:

∂F

∂Vf
=

1

tf − t0

∂F

∂V0
=
−1

tf − t0

∂F

∂tf
= − Vf − V0

(tf − t0)2

∂F

∂t0
=

Vf − V0

(tf − t0)2

Next, apply the general formula, (3), and drop the covariance terms (assumed to be zero).

σ2
F ≈

∣∣∣∣ ∂F∂Vf
∣∣∣∣2 σ2

V +

∣∣∣∣ ∂F∂V0

∣∣∣∣2 σ2
V +

∣∣∣∣∂F∂tf
∣∣∣∣2 σ2

t +

∣∣∣∣∂F∂t0
∣∣∣∣2 σ2

t

Finally, substitute and simplify:

σ2
F ≈

∣∣∣∣ 1

tf − t0

∣∣∣∣2 σ2
V +

∣∣∣∣ −1

tf − t0

∣∣∣∣2 σ2
V +

∣∣∣∣− Vf − V0

(tf − t0)2

∣∣∣∣2 σ2
t +

∣∣∣∣ Vf − V0

(tf − t0)2

∣∣∣∣2 σ2
t

≈ 2

(
1

tf − t0

)2

σ2
V + 2

(
Vf − V0

(tf − t0)2

)2

σ2
t

≈ 2

(
1

∆t

)2

σ2
V + 2

(
∆V

(∆t)2

)2

σ2
t

≈
(

∆V

∆t

)2 [
2
( σV

∆V

)2

+ 2
( σt

∆t

)2
]

≈ F 2

[
2
( σV

∆V

)2

+ 2
( σt

∆t

)2
]
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3 Calculation

Now that we have confirmed Approach 1 and Approach 2 yield the same error propagation
formula, we can perform the calculation. Recall the data for the first trial:

V0 t0 Vf tf

5.3 mL 1:01:04 49.2 mL 1:01:56

and our assumptions σV = 0.1 mL and σt = 1 s.

Calculate F and estimate σF :

F =
∆V

∆t
, σ2

F ≈ F 2

[
2
( σV

∆V

)2

+ 2
( σt

∆t

)2
]

∆V = Vf − V0 = 49.2− 5.3 = 43.9 mL

∆t = tf − t0 = 56− 4 = 52 s

F = 0.8442 mL/s

σF ≈ |F |
√

2
( σV

∆V

)2

+ 2
( σt

∆t

)2

≈ 0.0231 mL/s
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